theories/Monad.v
@@ -13,11 +13,12 @@ Arguments typ [_] _.
 Arguments mon [_ _ _] _.
 
 Record Weak (wl : wfLCon) (P : forall wl', wl' ≤ε wl  -> Type) : Type :=
-  { PN : nat ;
+  { WN : nat ;
     WP : forall (wl' : wfLCon) (alpha : wl' ≤ε wl),
-      AllInLCon PN wl' -> P wl' alpha ;
+      AllInLCon WN wl' -> P wl' alpha ;
   }.
-
+Arguments WN [_ _] _.
+Arguments WP [_ _] _ [_] _.
 
 Lemma monot (wl wl' wl'' : wfLCon)
   (P : forall wl',  wl' ≤ε wl -> Type)
@@ -30,8 +31,9 @@ Proof.
   exists N.
   intros wl''' dzeta allinl.
   exact (WN wl''' (dzeta •ε beta) allinl).
-Qed.  
+Qed.
 
+  
 
 Definition Wbind (wl : wfLCon) (P Q : forall wl', wl' ≤ε wl  -> Type)
   (Pe : forall wl' (alpha : wl' ≤ε wl) wl'' (beta : wl'' ≤ε wl),
@@ -40,24 +42,23 @@ Definition Wbind (wl : wfLCon) (P Q : forall wl', wl' ≤ε wl  -> Type)
       wl'' ≤ε wl' -> Q wl' alpha -> Q wl'' beta)
   (f : forall wl' (alpha : wl' ≤ε wl),
       P wl' alpha -> Weak wl' (fun wl'' beta => Q wl'' (beta •ε alpha))) :
-  forall wl' (alpha : wl' ≤ε wl),
-    Weak wl' (fun wl'' beta => P wl'' (beta •ε alpha)) ->
-    Weak wl' (fun wl'' beta => Q wl'' (beta •ε alpha)).
+    Weak wl (fun wl' beta => P wl' beta)->
+    Weak wl (fun wl' beta => Q wl' beta).
 Proof.
   intros * [N W].
   unshelve econstructor.
   { unshelve eapply (max N _).
     unshelve eapply Max_Bar.
-    - exact wl'.
+    - exact wl.
     - exact N.
-    - intros wl'' beta allinl.
-      unshelve eapply (f wl'' (beta •ε alpha)).
+    - intros wl' alpha allinl.
+      unshelve eapply (f wl' alpha).
       now eapply W.
   }
-  intros wl'' beta allinl.
+  intros wl' alpha allinl.
   unshelve eapply Qe.
   4: unshelve eapply f.
-  { unshelve eapply (Bar_lub (Bar_lub wl' wl'' N beta _) wl'').
+  { unshelve eapply (Bar_lub (Bar_lub wl wl' N alpha _) wl').
     3: now eapply Bar_lub_smaller.
     3: eassumption.
     eapply AllInLCon_le.
@@ -65,10 +66,9 @@ Proof.
     eassumption.
   }
   + unshelve eapply Bar_lub_smaller.
-  + eapply (Bar_lub wl' wl'' N beta _).
+  + eapply (Bar_lub wl wl' N alpha _).
   + now eapply Bar_lub_ub.
-  + unshelve eapply (_ •ε alpha).
-    now eapply Bar_lub_ub.
+  + now eapply Bar_lub_ub.
   + eapply W.
     now eapply Bar_lub_AllInLCon.
   + eapply AllInLCon_le ; [ | now eapply Bar_lub_AllInLCon].
@@ -88,6 +88,32 @@ Proof.
   - exact 0.
   - intros ; now eapply Pe.
 Defined.
+
+Definition WFunEq (wl : wfLCon)
+  (LRP : forall wl', wl' ≤ε wl  -> Type)
+  (LRQ : forall wl' (alpha : wl' ≤ε wl),
+      LRP wl' alpha -> Type)
+  (p : Weak wl LRP) : Type :=
+  forall wl' (α : wl' ≤ε wl) (allinl : AllInLCon p.(WN) wl'),
+    LRQ wl' α (p.(WP) α allinl).
+
+(*Definition WFuncTy (wl : wfLCon)
+  (LRDelta : forall wl', wl' ≤ε wl  -> Type)
+  (LRP : forall wl' (alpha : wl' ≤ε wl),
+      LRDelta wl' alpha -> Type)
+  (LRA : forall wl' alpha delta,
+      LRP wl' alpha delta -> Type)
+  (LRQ : forall wl' alpha delta (p : LRP wl' alpha delta),
+      LRA wl' alpha delta p ->
+      forall wl'', wl'' ≤ε wl' -> Type)
+  (p : Weak wl (fun wl' alpha => forall delta, LRP wl' alpha delta)) :
+  Type :=
+  forall (wl' : wfLCon) (alpha : wl' ≤ε wl)
+         (delta : LRDelta wl' alpha)
+         (allinl : AllInLCon p.(WN) wl')
+         (Ha : LRA wl' alpha delta (p.(WP) alpha allinl delta)),
+    Weak wl' (LRQ wl' alpha delta (p.(WP) alpha allinl delta) Ha).
+*)
 
 
 (*
